

1. For every $a, b, c \in \mathbb{N}$, $\text{lcm}(ca, cb) = c \cdot \text{lcm}(a, b)$.

Proof. Let $a, b, c \in \mathbb{N}$, $m = \text{lcm}(ca, cb)$, and $n = c \cdot \text{lcm}(a, b)$. To show that $m = n$, we will show that $m \leq n$ and $n \leq m$.

Since $m = \text{lcm}(ca, cb)$, by the definition of least common multiple, we know there exist integers k_1 and k_2 such that

$$cak_1 = m = cbk_2.$$

Since $c \neq 0$, we can divide each equation above to obtain

$$ak_1 = \frac{m}{c} = bk_2,$$

where we know k_1 , k_2 , and $\frac{m}{c}$ are all integers. Thus, we have shown that $\frac{m}{c}$ is a common multiple of a and b . By the definition of least common multiple, we know $\text{lcm}(a, b) \leq \frac{m}{c}$. Multiplying the previous inequality by c gives

$$n = c \cdot \text{lcm}(a, b) \leq c \cdot \frac{m}{c} = m,$$

and we conclude that $n \leq m$.

To show the reverse inequality, we apply the definition of least common multiple to $\text{lcm}(a, b)$ to conclude that there exist integers k_1 and k_2 such that

$$ak_1 = \text{lcm}(a, b) = bk_2.$$

Multiplying both equations by c , we obtain

$$cak_1 = c \cdot \text{lcm}(a, b) = cbk_2.$$

Thus, we have shown that $c \cdot \text{lcm}(a, b)$ is a common multiple of both ca and cb . Thus,

$$m = \text{lcm}(ca, cb) \leq c \cdot \text{lcm}(a, b) = n.$$

□

2. Every multiple of 4 can be written in the form $1 + (-1)^n(2n - 1)$ for some $n \in \mathbb{N}$.

Proof. Let $m = 4a$ where $a \in \mathbb{Z}$. We will proceed by cases based on the value of a .

Case 1: Suppose $a = 0$.

Choose $n = 1$. Observe $1 \in \mathbb{N}$. Now, $1 + (-1)^n(2n - 1) = 1 - 1 = 0 = 4 \cdot 0$, which is what we needed to show.

Case 2: Suppose $a > 0$.

Choose $n = 2a$. Observe that since $a \in \mathbb{N}$, we know $n = 2a \in \mathbb{N}$. Now, $1 - (-1)^n(2n - 1) = 1 + (4a - 1) = 4a$, which is what we needed to show.

Case 3: Suppose $a < 0$.

Choose $n = -2a + 1$. Observe that since a is a negative integer, $2a + 1 \in \mathbb{N}$. Now, $1 - (-1)^n(2n - 1) = 1 - (2(-2a + 1) - 1) = 1 - (-4a + 2 - 1) = 4a$, which is what we needed to show.

□

3. For every integer n , $n^2 + 3n + 3$ is odd.

Proof. We will proceed by cases depending on the parity of n .

Case 1: Suppose n is even.

By definition of even, there is an integer k such that $n = 2k$. Thus,

$$n^2 + 3n + 3 = (2k)^2 + 3(2k) + 3 = 2(2k^2 + 3k + 1) + 1.$$

Since k is an integer, Fact 4.1 implies that $\ell = 2k^2 + 3k + 1$ is also an integer. Thus, we have shown that when n is even, $n^2 + 3n + 3 = 2\ell + 1$, where $\ell \in \mathbb{Z}$. Thus, $n^2 + 3n + 3$ is even by definition in this case.

Case 2: Suppose n is odd.

By definition of odd, there is an integer k such that $n = 2k + 1$. Thus,

$$n^2 + 3n + 3 = (2k + 1)^2 + 3(2k + 1) + 3 = 2(2k^2 + 5k + 3) + 1.$$

Since k is an integer, Fact 4.1 implies that $\ell = 2k^2 + 5k + 3$ is also an integer. Thus, we have shown that when n is odd, $n^2 + 3n + 3 = 2\ell + 1$, where $\ell \in \mathbb{Z}$. Thus, $n^2 + 3n + 3$ is even by definition in this case.

□

4. Let $a, b \in \mathbb{N}$. If $\gcd(a, b) > 1$, then $b \mid a$ or b is not prime.

Proof. Let $a, b \in \mathbb{N}$ such that $\gcd(a, b) > 1$. We will proceed by cases based on whether or not b is prime.

Case 1: b is not prime.

Then the result follows immediately.

Case 2: b is prime.

Since b is prime, its only divisors are 1 and b . Thus, $\gcd(a, b) \in \{1, b\}$. But $\gcd(a, b) > 1$. Thus, $\gcd(a, b) \neq 1$ and therefore $\gcd(a, b) = b$. Since $\gcd(a, b) \mid a$ and $\gcd(a, b) = b$, it follows that $b \mid a$. \square